LeanYjs/YjsArray.lean
@@ -1,0 +1,473 @@
+import LeanYjs.Item
+import LeanYjs.ItemSet
+import LeanYjs.ActorId
+import LeanYjs.ItemOrder
+import LeanYjs.ItemSetInvariant
+import LeanYjs.Totality
+import LeanYjs.Transitivity
+import LeanYjs.AntiSymmetry
+import LeanYjs.Integrate
+
+variable {A : Type}
+variable [BEq A]
+
+def ArrSet (arr : List (YjsItem A)) : YjsPtr A -> Prop :=
+  fun a => match a with
+  | YjsPtr.itemPtr item => item ∈ arr
+  | YjsPtr.first => True
+  | YjsPtr.last => True
+
+def ArrSetClosed (arr : List (YjsItem A)) : Prop :=
+  IsClosedItemSet (ArrSet arr)
+
+omit [BEq A] in lemma arr_set_closed_push (arr : List (YjsItem A)) (item : YjsItem A) :
+  ArrSetClosed arr ->
+  ArrSet arr item.origin ->
+  ArrSet arr item.rightOrigin ->
+  ArrSetClosed (item :: arr) := by
+  intros hclosed horigin hright
+  constructor <;> try simp [ArrSet, IsClosedItemSet]
+  . intros o r id c hor
+    cases o with
+    | itemPtr item' =>
+      simp
+      cases hor with
+      | inr hitem =>
+        right
+        apply hclosed.closedLeft at hitem
+        assumption
+      | inl heq =>
+        subst heq
+        right
+        assumption
+    | first =>
+      simp
+    | last =>
+      simp
+  . intros o r id c hor
+    cases r with
+    | itemPtr item' =>
+      simp
+      cases hor with
+      | inr hitem =>
+        right
+        apply hclosed.closedRight at hitem
+        assumption
+      | inl heq =>
+        subst heq
+        right
+        assumption
+    | first =>
+      simp
+    | last =>
+      simp
+
+omit [BEq A] lemma yjs_lt_mono (P Q : ItemSet A) (x y : YjsPtr A) :
+  IsClosedItemSet P ->
+  ItemSetInvariant P ->
+  (∀ a, P a -> Q a) ->
+  YjsLt P h x y ->
+  YjsLt Q h x y := by
+  intros hclosedP hinvP hsubset
+  intros hlt
+  revert hlt x y
+  apply Nat.strongRec' (p := fun h => ∀ x y, YjsLt P h x y → YjsLt Q h x y)
+  intros n ih x y hlt
+  cases hlt with
+  | ltOriginOrder _  _ _ _ hlt =>
+    apply YjsLt.ltOriginOrder
+    . apply hsubset ; assumption
+    . apply hsubset ; assumption
+    . assumption
+  | ltConflict _ _ _ hlt =>
+    cases hlt with
+    | ltOriginDiff =>
+      apply YjsLt.ltConflict
+      apply ConflictLt.ltOriginDiff
+      all_goals (apply ih; unfold max4; omega)
+      all_goals (assumption)
+    | ltOriginSame =>
+      apply YjsLt.ltConflict
+      apply ConflictLt.ltOriginSame <;> try assumption
+      all_goals (apply ih; omega)
+      all_goals (assumption)
+  | ltOrigin _ _ _ _ _ _ _ hlt =>
+    apply YjsLt.ltOrigin
+    . apply hsubset ; assumption
+    . cases hlt with
+      | leqSame =>
+        apply YjsLeq.leqSame
+        apply hsubset ; assumption
+      | leqLt =>
+        apply YjsLeq.leqLt
+        apply ih <;> try assumption
+        omega
+  | ltRightOrigin _ _ _ _ _ _ _ hlt =>
+    apply YjsLt.ltRightOrigin
+    . apply hsubset ; assumption
+    . cases hlt with
+      | leqSame =>
+        apply YjsLeq.leqSame
+        apply hsubset ; assumption
+      | leqLt =>
+        apply YjsLeq.leqLt
+        apply ih <;> try assumption
+        omega
+
+lemma yjs_lt'_mono :
+  ∀ (P Q : ItemSet A) (x y : YjsPtr A),
+  IsClosedItemSet P ->
+  ItemSetInvariant P ->
+  (∀ a, P a -> Q a) ->
+  YjsLt' P x y -> YjsLt' Q x y := by
+  intros P Q x y hclosedP hinvP hsubset hlt
+  obtain ⟨ _, hlt ⟩ := hlt
+  constructor
+  apply yjs_lt_mono P Q x y hclosedP hinvP hsubset hlt
+
+lemma yjs_leq'_mono :
+  ∀ (P Q : ItemSet A) (x y : YjsPtr A),
+  IsClosedItemSet P ->
+  ItemSetInvariant P ->
+  (∀ a, P a -> Q a) ->
+  YjsLeq' P x y -> YjsLeq' Q x y := by
+  intros P Q x y hclosedP hinvP hsubset hleq
+  obtain ⟨ _, hleq ⟩ := hleq
+  cases hleq with
+  | leqSame =>
+    exists 0
+    apply YjsLeq.leqSame
+    apply hsubset; assumption
+  | leqLt =>
+    constructor
+    apply YjsLeq.leqLt
+    apply yjs_lt_mono P Q x y hclosedP hinvP hsubset
+    assumption
+
+lemma push_subset {A} (arr : List (YjsItem A)) (a : YjsItem A) :
+  ∀ x, ArrSet arr x -> ArrSet (a :: arr) x := by
+  intros x hin
+  unfold ArrSet at *
+  simp
+  cases x <;> (simp at *)
+  right; assumption
+
+lemma reachable_in {A} (arr : List (YjsItem A)) (a : YjsPtr A) :
+  IsClosedItemSet (ArrSet arr) ->
+  ∀ x, OriginReachable a x -> ArrSet arr a -> ArrSet arr x := by
+  intros hclosed x hreach hin
+  induction hreach with
+  | reachable_head x a y step h ih =>
+    cases step with
+    | reachable =>
+      simp [ArrSet] at hin
+      apply hclosed.closedLeft at hin
+      apply ih
+      assumption
+    | reachable_right =>
+      simp [ArrSet] at hin
+      apply hclosed.closedRight at hin
+      apply ih
+      assumption
+  | reachable_single _ _ hstep =>
+    cases hstep with
+    | reachable =>
+      simp [ArrSet] at hin
+      apply hclosed.closedLeft at hin
+      assumption
+    | reachable_right =>
+      simp [ArrSet] at hin
+      apply hclosed.closedRight at hin
+      assumption
+
+lemma item_set_invariant_push (arr : List (YjsItem A)) (item : YjsItem A) :
+  ItemSetInvariant (ArrSet arr) ->
+  ArrSetClosed arr ->
+  YjsLt' (ArrSet arr) item.origin item.rightOrigin ->
+  (∀ x, OriginReachable item x -> YjsLeq' (ArrSet arr) x item.origin ∨ YjsLeq' (ArrSet arr) item.rightOrigin x) ->
+  (∀ x : YjsItem A, ArrSet arr x -> x.id = item.id -> YjsLeq' (ArrSet arr) x item.origin ∨ YjsLeq' (ArrSet arr) item.rightOrigin x) ->
+  ItemSetInvariant (ArrSet (item :: arr)) := by
+  intros hinv hclosed horigin hreach hsameid
+  apply ItemSetInvariant.mk
+  . intros o r c id hitem
+    simp [ArrSet] at hitem
+    cases hitem with
+    | inr hin =>
+      apply hinv.origin_not_leq at hin
+      apply yjs_lt'_mono _ _ _ _  hclosed hinv _ hin
+      . intros a hlt
+        simp [ArrSet] at *
+        cases a <;> simp at *
+        right; assumption
+    | inl heq =>
+      subst heq
+      simp [YjsItem.origin, YjsItem.rightOrigin] at horigin
+      apply yjs_lt'_mono _ _ _ _  hclosed hinv _ horigin
+      . intros a hlt
+        simp [ArrSet] at *
+        cases a <;> simp at *
+        right; assumption
+  . intros o r c id x hin hreachable
+    simp [ArrSet] at hin
+    cases hin with
+    | inr hin =>
+      obtain hor := hinv.origin_nearest_reachable _ _ _ _ _ hin hreachable
+      cases hor with
+      | inl hor =>
+        left
+        apply yjs_leq'_mono _ _ _ _ hclosed hinv _ hor
+        intros
+        apply push_subset; assumption
+      | inr hor =>
+        right
+        apply yjs_leq'_mono _ _ _ _ hclosed hinv _ hor
+        intros
+        apply push_subset; assumption
+    | inl heq =>
+      subst heq
+      simp [YjsItem.origin, YjsItem.rightOrigin] at *
+      cases hreach _ hreachable with
+      | inl hor =>
+        left
+        apply yjs_leq'_mono _ _ _ _ hclosed hinv _ hor
+        intros
+        apply push_subset; assumption
+      | inr hor =>
+        right
+        apply yjs_leq'_mono _ _ _ _ hclosed hinv _ hor
+        intros
+        apply push_subset; assumption
+  . intros x y hinx hiny hineq hid
+    simp [ArrSet] at *
+    cases hinx with
+    | inr hinx =>
+      cases hiny with
+      | inr hiny =>
+        obtain hor := hinv.same_id_ordered _ _ hinx hiny hineq hid
+        cases hor with
+        | inl hleq =>
+          left
+          apply yjs_leq'_mono _ _ _ _ hclosed hinv _ hleq
+          apply push_subset
+        | inr hleq =>
+          right
+          cases hleq with
+          | inl hleq =>
+            left
+            apply yjs_leq'_mono _ _ _ _ hclosed hinv _ hleq
+            apply push_subset
+          | inr hleq =>
+            right
+            cases hleq with
+            | inl hleq =>
+              left
+              apply yjs_leq'_mono _ _ _ _ hclosed hinv _ hleq
+              apply push_subset
+            | inr hleq =>
+              right
+              apply yjs_leq'_mono _ _ _ _ hclosed hinv _ hleq
+              apply push_subset
+      | inl hleq =>
+        subst hleq
+        cases hsameid _ hinx hid with
+        | inl hleq =>
+          left
+          apply yjs_leq'_mono _ _ _ _ hclosed hinv _ hleq
+          apply push_subset
+        | inr hleq =>
+          right
+          right
+          right
+          apply yjs_leq'_mono _ _ _ _ hclosed hinv _ hleq
+          apply push_subset
+    | inl hinx =>
+      subst hinx
+      cases hiny with
+      | inr hiny =>
+        cases hsameid _ hiny (by rw [hid]) with
+        | inl hleq =>
+          right
+          left
+          apply yjs_leq'_mono _ _ _ _ hclosed hinv _ hleq
+          apply push_subset
+        | inr hleq =>
+          right
+          right
+          left
+          apply yjs_leq'_mono _ _ _ _ hclosed hinv _ hleq
+          apply push_subset
+      | inl heqy =>
+        subst heqy
+        cases hineq (refl _)
+
+structure YjsArrInvariant (arr : List (YjsItem A)) : Prop where
+  closed : IsClosedItemSet (ArrSet arr)
+  item_set_inv : ItemSetInvariant (ArrSet arr)
+  sorted : List.Pairwise (fun (x y : YjsItem A) => YjsLt' (ArrSet arr) x y) arr
+  unique : List.Pairwise (fun x y => x ≠ y) arr
+
+lemma same_yjs_set_unique_aux (xs_all ys_all xs ys : List (YjsItem A)) :
+  YjsArrInvariant xs_all ->
+  YjsArrInvariant ys_all ->
+  (∀ a, ArrSet xs_all a ↔ ArrSet ys_all a) ->
+  (∃ t, t ++ xs = xs_all) ->
+  (∃ t, t ++ ys = ys_all) ->
+  (∀ x, ArrSet xs x ↔ ArrSet ys x) ->
+  xs = ys := by
+  intros hinv1 hinv2 hseteq_all hsubset1 hsubset2 hseteq
+  obtain ⟨ hclosed1, hinv1, hsort1, huniq1 ⟩ := hinv1
+  obtain ⟨ hclosed2, hinv2, hsort2, huniq2 ⟩ := hinv2
+
+  revert ys
+
+  induction xs with
+  | nil =>
+    intros ys hsubset2 hseteq
+    cases ys with
+    | nil => eq_refl
+    | cons y ys =>
+      obtain hitem := hseteq y
+      simp [ArrSet] at hitem
+  | cons x xs ih =>
+    intros ys hsubset2 hseteq
+    cases ys with
+    | nil =>
+      obtain hitem := hseteq x
+      simp [ArrSet] at hitem
+    | cons y ys =>
+      have hmin1 : ∀ a ∈ xs, YjsLt' (ArrSet xs_all) x a := by
+        obtain ⟨ t, heq ⟩ := hsubset1
+        subst heq
+        rw [List.pairwise_append] at hsort1
+        obtain ⟨ _, hsort1, _ ⟩ := hsort1
+        simp at hsort1
+        obtain ⟨ hsort1, _ ⟩ := hsort1
+        assumption
+      have hmin2 : ∀ a ∈ ys, YjsLt' (ArrSet ys_all) y a := by
+        obtain ⟨ t, heq ⟩ := hsubset2
+        subst heq
+        rw [List.pairwise_append] at hsort2
+        obtain ⟨ _, hsort2, _ ⟩ := hsort2
+        simp at hsort2
+        obtain ⟨ hsort2, _ ⟩ := hsort2
+        assumption
+
+      have heq : x = y := by
+        have hlt1 : x = y ∨ YjsLt' (ArrSet ys_all) y x := by
+          cases yjsItem_decidable_eq A x y with
+          | inl heq =>
+            left; assumption
+          | inr hneq =>
+            obtain ⟨ hinx, _ ⟩ := hseteq x
+            have hinx : x = y ∨ x ∈ ys:= by
+              simp [ArrSet] at hinx
+              assumption
+            cases hinx with
+            | inl heq =>
+              left; assumption
+            | inr hinx =>
+              apply hmin2 at hinx
+              obtain ⟨ _, hinx ⟩ := hinx
+              right
+              constructor
+              assumption
+
+        have hlt2 : x = y ∨ YjsLt' (ArrSet xs_all) x y := by
+          cases yjsItem_decidable_eq A x y with
+          | inl heq =>
+            subst heq; left; eq_refl
+          | inr hneq =>
+            obtain ⟨ _, hinx ⟩ := hseteq y
+            have hiny : y = x ∨ y ∈ xs:= by
+              simp [ArrSet] at hinx
+              assumption
+            cases hiny with
+            | inl heq =>
+              subst heq; left; eq_refl
+            | inr hiny =>
+              apply hmin1 at hiny
+              obtain ⟨ _, hiny ⟩ := hiny
+              right
+              constructor
+              assumption
+
+        cases hlt1 with
+        | inl heq =>
+          assumption
+        | inr hlt1 =>
+          cases hlt2 with
+          | inl heq =>
+            assumption
+          | inr hlt2 =>
+            have hlt3 : YjsLt' (ArrSet ys_all) x y := by
+              apply yjs_lt'_mono (ArrSet xs_all) _ _ _ hclosed1 hinv1 <;> try assumption
+              intros a hlt
+              rw [<-hseteq_all a]; assumption
+
+            cases yjs_lt_anti_symm hclosed2 hinv2 x y hlt3 hlt1
+
+      subst heq
+      congr
+
+      apply ih
+      . obtain ⟨ t, heq ⟩ := hsubset1
+        subst heq
+        exists (t ++ [x])
+        simp
+      . obtain ⟨ t, heq ⟩ := hsubset2
+        subst heq
+        exists (t ++ [x])
+        simp
+      . intros a
+        simp [ArrSet] at *
+        cases a with
+        | first =>
+          simp
+        | last =>
+          simp
+        | itemPtr a =>
+          specialize hseteq a
+          simp at *
+          obtain ⟨ t, heq ⟩ := hsubset1
+          subst heq
+          obtain ⟨ t', heq ⟩ := hsubset2
+          subst heq
+          rw [List.pairwise_append] at huniq1
+          rw [List.pairwise_append] at huniq2
+          simp at *
+          obtain ⟨ _, ⟨ huniq1, _ ⟩, _ ⟩ := huniq1
+          obtain ⟨ _, ⟨ huniq2, _ ⟩ , _ ⟩ := huniq2
+          constructor
+          . intros hin
+            obtain hneq := huniq1 _ hin
+            have h : a = x ∨ a ∈ ys := by
+              rw [<-hseteq]
+              right; assumption
+            cases h with
+            | inl heq =>
+              subst heq
+              cases hneq (refl _)
+            | inr hin =>
+              assumption
+          . intros hin
+            obtain hneq := huniq2 _ hin
+            have h : a = x ∨ a ∈ xs := by
+              rw [hseteq]
+              right; assumption
+            cases h with
+            | inl heq =>
+              subst heq
+              cases hneq (refl _)
+            | inr hin =>
+              assumption
+
+lemma same_yjs_set_unique (xs ys : List (YjsItem A)) :
+  YjsArrInvariant xs ->
+  YjsArrInvariant ys ->
+  (∀ a, ArrSet xs a ↔ ArrSet ys a) ->
+  xs = ys := by
+  intros hinv1 hinv2 hseteq
+  apply same_yjs_set_unique_aux xs ys xs ys hinv1 hinv2 hseteq
+  . exists []
+  . exists []
+  . apply hseteq
